vale/code/arch/x64/X64.Stack_i.fsti
@@ -98,9 +98,8 @@ val lemma_correct_store_load_taint_stack64: (ptr:int) -> (t:taint) -> (stackTain
   [SMTPat (valid_taint_stack64 ptr t (store_taint_stack64 ptr t stackTaint))]
 
 val lemma_frame_store_load_taint_stack64: (ptr:int) -> (t:taint) -> (stackTaint:memtaint) -> (i:int) -> (t':taint) -> Lemma
-  (requires valid_taint_stack64 i t' stackTaint /\
-    (i >= ptr + 8 \/ i + 8 <= ptr))
-  (ensures (valid_taint_stack64 i t' (store_taint_stack64 ptr t stackTaint)))
+  (requires i >= ptr + 8 \/ i + 8 <= ptr)
+  (ensures valid_taint_stack64 i t' stackTaint == valid_taint_stack64 i t' (store_taint_stack64 ptr t stackTaint))
   [SMTPat (valid_taint_stack64 i t' (store_taint_stack64 ptr t stackTaint))]
 
 
@@ -112,3 +111,8 @@ let valid_stack_slot64s (base num_slots:nat) (h:stack) (t:taint) (stackTaint:mem
     (valid_stack_slot64 addr h t stackTaint)}
     (base <= addr) && (addr < base + num_slots `op_Multiply` 8) && (addr - base) % 8 = 0 ==>
       valid_src_stack64 addr h /\ valid_taint_stack64 addr t stackTaint
+
+let modifies_stacktaint (lo_rsp hi_rsp:nat) (h h':memtaint) : Prop_s.prop0 =
+  forall addr t. {:pattern (valid_taint_stack64 addr t h') }
+    (addr + 8 <= lo_rsp || addr >= hi_rsp) ==>
+      valid_taint_stack64 addr t h == valid_taint_stack64 addr t h'
